\subsubsection*{A solution}

By definition of $Y$,

\begin{align*}
F_Y(y) &= P_Y(Y \leq y) \\
&= P_X( -\frac{1}{\lambda} \log X \leq y) \\
&= P_X(\log X \geq -\lambda y) \text{, since $\lambda > 0$} \\
&= P_X(X \geq \exp(-\lambda y)) \text{, since $\exp$ preserves ordering on $\mathbb{R}$}
\end{align*}

The probability density function of $U(a, b)$ is $\frac{1}{b-a} \cdot I_{s \in[a, b]}$, where here we mean $I$ as the indicator function ($=1$ for $s \in [a, b]$, otherwise 0).
Thus we have

\begin{align*}
F_Y(y) &= \int_{\exp(-\lambda y)}^{\infty} \frac{1}{b-a} \cdot I_{s \in[a, b]} ds \\
&= \frac{1}{b - a} \int_{\exp(-\lambda y)}^{\infty} I_{s \in[a, b]} ds
\end{align*}

We consider now cases on $y$ values.
If $\exp(-\lambda y) > b$, we have $F_Y(y) =0 $. This condition is equivalent to
\begin{align*}
    &-\lambda y > \log(b), \text { since $\log$ preserves ordering on $\mathbb{R}$, and} \\
    &y < - \frac{1}{\lambda} \log(b), \text{ since $\lambda > 0$.}
\end{align*}

Next, if $ - \frac{1}{\lambda} \log(b) \leq y \leq - \frac{1}{\lambda} \log(a)$, we have $F_Y(y) = \frac{b - \exp(-\lambda y)}{b - a}$.

Finally, if $y > - \frac{1}{\lambda} \log(a)$, then the integral evaluates to $b - a$, and $F_Y(y) = 1$ for such $y$ values.


Putting the pieces together,

\begin{equation}
F_Y(y)=
    \begin{cases}
        0 & \text{if } y < -\frac{1}{\lambda} \log(b) \\
        \frac{b - \exp(-\lambda y)}{b - a} & \text{if }- \frac{1}{\lambda} \log(b) \leq y \leq - \frac{1}{\lambda} \log(a) \\
        1 & \text {if } y > - \frac{1}{\lambda} \log(a).
    \end{cases}
\end{equation}

The resulting  $Y$ is called a truncated exponential distribution.
